
module Verification.Core.Syntax.SignatureZ3 where

open import Verification.Conventions hiding (k)
open import Verification.Core.Category
open import Verification.Core.Order
open import Verification.Core.Type
open import Verification.Core.Category.Monad
open import Verification.Core.Category.Instance.Kleisli
open import Verification.Core.Category.Instance.IdxSet
open import Verification.Core.Category.Limit.Specific
open import Verification.Core.Category.Limit.Kan
-- open import Verification.Unification.RecAccessible


module _ {K : 𝒰₀} where
  -- Symbol : 𝒰₀
  -- Symbol = ∑ λ (n : ℕ) -> K ×-𝒰 (Vec K n)

  Signature : 𝒰₁
  Signature = {n : ℕ} -> K -> Vec K (suc n) -> 𝒰₀

  isInhabited-Sig : Signature -> 𝒰₀
  isInhabited-Sig σ = ∀ k -> ∑ λ n -> ∑ λ (ks : Vec K (suc n)) -> σ k ks

  data TermO (σ : Signature) (V : K -> 𝒰₀) (k : K) : 𝒰₀
  data TermsO (σ : Signature) (V : K -> 𝒰₀) : {n : ℕ} (ks : Vec K n) -> 𝒰₀ where
    [] : TermsO σ V []
    _∷_ : ∀{k} {ks : Vec K n} -> (t : TermO σ V k) -> (ts : TermsO σ V ks) -> TermsO σ V (k ∷ ks)

  data TermO σ V k where
    te : ∀{ks : Vec K (suc n)} -> (s : σ k ks) -> (ts : TermsO σ V ks) -> TermO σ V k
    var : V k -> TermO σ V k
    fail : TermO σ V k

  data Term (σ : Signature) (V : K -> 𝒰₀) (k : K) : 𝒰₀
  data Terms (σ : Signature) (V : K -> 𝒰₀) : {n : ℕ} (ks : Vec K n) -> 𝒰₀ where
    [] : Terms σ V []
    _∷_ : ∀{k} {ks : Vec K n} -> (t : Term σ V k) -> (ts : Terms σ V ks) -> Terms σ V (k ∷ ks)

  -- data isNotFail-Term {σ : Signature} {V : K -> 𝒰₀} : {k : K} -> Term σ V k -> 𝒰₀ where
  data Termᵥ (σ : Signature) (V : K -> 𝒰₀) (k : K) : 𝒰₀

  -- data isNotFail-Terms {σ : Signature} {V : K -> 𝒰₀} : {n : ℕ} {ks : Vec K n} -> Terms σ V ks -> 𝒰₀
  data Termsᵥ (σ : Signature) (V : K -> 𝒰₀) : {n : ℕ} (ks : Vec K n) -> 𝒰₀

  data Term σ V k where
    te : ∀{ks : Vec K (suc n)} -> (s : σ k ks) -> (ts : Termsᵥ σ V ks) -> Term σ V k
    var : V k -> Term σ V k
    fail : Term σ V k

  data Termsᵥ σ V where
    _∷_ : {k : K} -> (Termᵥ σ V k) -> ∀{n} -> {ks : Vec K n} -> (ts : Terms σ V ks) -> Termsᵥ σ V (k ∷ ks)
    fail∷_ : {k : K} -> {ks : Vec K n} -> (ts : Termsᵥ σ V ks) -> Termsᵥ σ V (k ∷ ks)

  data Termᵥ σ V k where
    te : ∀{ks : Vec K (suc n)} -> (s : σ k ks) -> (ts : Termsᵥ σ V ks) -> Termᵥ σ V k
    var : V k -> Termᵥ σ V k


  module _ {σ : Signature} {V : K -> 𝒰₀} where
    forget-Term : ∀{k} -> Termᵥ σ V k -> Term σ V k
    forget-Term (te s ts) = te s ts
    forget-Term (var x) = var x

    forget-Terms : {ks : Vec K n} -> Termsᵥ σ V ks -> Terms σ V ks
    forget-Terms (x ∷ ts) = forget-Term x ∷ ts
    forget-Terms (fail∷ ts) = fail ∷ forget-Terms ts

    split:∷ᵥ : {k : K} -> {t s : Termᵥ σ V k} -> ∀{n} -> {ks : Vec K n} -> {u v : Terms σ V ks}
            -> StrId {A = Termsᵥ σ V (k ∷ ks)} (t ∷ u) (s ∷ v) -> (t ≡-Str s) ×-𝒰 (u ≡-Str v)
    split:∷ᵥ refl-StrId = refl , refl

    split:∷ : {k : K} -> {t s : Term σ V k} -> ∀{n} -> {ks : Vec K n} -> {u v : Terms σ V ks}
            -> StrId {A = Terms σ V (k ∷ ks)} (t ∷ u) (s ∷ v) -> (t ≡-Str s) ×-𝒰 (u ≡-Str v)
    split:∷ refl-StrId = refl , refl

    isInjective:forget-Term : ∀{k} -> {t s : Termᵥ σ V k} -> forget-Term t ≡-Str forget-Term s -> t ≡-Str s
    isInjective:forget-Term {t = te s₁ ts} {te .s₁ .ts} refl-StrId = refl-StrId
    isInjective:forget-Term {t = var x} {var .x} refl-StrId = refl-StrId

    isInjective:forget-Terms : {ks : Vec K n} -> {t s : Termsᵥ σ V ks} -> forget-Terms t ≡-Str forget-Terms s -> t ≡-Str s
    isInjective:forget-Terms {t = x ∷ ts} {x₁ ∷ ts₁} p with split:∷ p
    ... | p1 , refl-StrId with isInjective:forget-Term p1
    ... | refl-StrId = refl
    isInjective:forget-Terms {t = x ∷ ts} {fail∷ s} p with split:∷ p
    isInjective:forget-Terms {suc _} {_ ∷ _} {te s₁ ts₁ ∷ ts} {fail∷ s} p | () , p2
    isInjective:forget-Terms {suc _} {_ ∷ _} {var x ∷ ts} {fail∷ s} p | () , p2
    isInjective:forget-Terms {t = fail∷ t} {x ∷ ts} p with split:∷ p
    isInjective:forget-Terms {suc _} {_ ∷ _} {fail∷ t} {te s ts₁ ∷ ts} p | () , p2
    isInjective:forget-Terms {suc _} {_ ∷ _} {fail∷ t} {var x ∷ ts} p | () , p2
    isInjective:forget-Terms {t = fail∷ t} {fail∷ s} p with split:∷ p
    ... | p1 , p2 with isInjective:forget-Terms p2
    ... | refl-StrId = refl-StrId

  module _ {σ : Signature} {V : K -> 𝒰₀} where
    data isFail-Term {k : K} : (Term σ V k) -> 𝒰₀ where
      fail : isFail-Term fail

    cast::isFail-Term : {k : K} -> {t : Term σ V k} -> isFail-Term t -> t ≡ fail
    cast::isFail-Term fail = refl

    data isFail-Terms : {n : ℕ} {ks : Vec K n} -> (ts : Terms σ V ks) -> 𝒰₀ where
      [] : isFail-Terms []
      _∷_ : ∀{k} -> {t : Term σ V k} -> (isFail-Term t) -> {n : ℕ} {ks : Vec K n} -> {ts : Terms σ V ks} -> isFail-Terms ts -> isFail-Terms (t ∷ ts)

    data _⊏-Terms_ : {k : K} -> ∀{n} -> {ks : Vec K n} -> (t : Term σ V k) -> (ts : Terms σ V ks) -> 𝒰₀ where
      this : {k : K} -> {t : Term σ V k} -> ∀{n} -> {ks : Vec K n} -> {ts : Terms σ V ks} -> t ⊏-Terms (t ∷ ts)
      _∷_ : {k₁ k₂ : K} -> {t₁ : Term σ V k₁} -> (t₂ : Term σ V k₂)-> ∀{n} -> {ks : Vec K n} -> {ts : Terms σ V ks} -> t₁ ⊏-Terms ts -> t₁ ⊏-Terms (t₂ ∷ ts)

    -- data _⊏-Termsᵥ_ : {k : K} -> ∀{n} -> {ks : Vec K n} -> (t : Term σ V k) -> (ts : Termsᵥ σ V ks) -> 𝒰₀ where
    --   this : {k : K} -> (t : Termᵥ σ V k) -> (t' : Term σ V k) -> (forget-Term t ≡-Str t') -> ∀{n} -> {ks : Vec K n} -> {ts : Terms σ V ks} -> t' ⊏-Termsᵥ (t ∷ ts)
    --   older : {k₁ k₂ : K} -> {t₁ : Term σ V k₁} -> (t₂ : Termᵥ σ V k₂) -> ∀{n} -> {ks : Vec K n} -> {ts : Terms σ V ks} -> t₁ ⊏-Terms ts -> t₁ ⊏-Termsᵥ (t₂ ∷ ts)
    --   fail∷_ : ∀ {k} -> {k₁ : K} -> {t₁ : Term σ V k₁} -> ∀{n} -> {ks : Vec K n} -> {ts : Termsᵥ σ V ks} -> t₁ ⊏-Termsᵥ ts -> t₁ ⊏-Termsᵥ (fail∷_ {k = k} ts)

    data _⊏_ : {k₁ k₂ : K} -> (t₁ : Term σ V k₁) -> (t₂ : Term σ V k₂) -> 𝒰₀ where
      te : {k j : K} -> {t : Term σ V k} -> ∀{n} -> {ks : Vec K (suc n)} -> {s : σ j ks} -> {ts : Termsᵥ σ V ks} -> (t ⊏-Terms (forget-Terms ts)) -> t ⊏ te s (ts)
      fail : ∀{k j : K} -> {t : Term σ V k} -> (t ≢-Str fail) -> fail {k = j} ⊏ t

    -- data _⊏-TermsO_ : {k : K} -> ∀{n} -> {ks : Vec K n} -> (t : TermO σ V k) -> (ts : TermsO σ V ks) -> 𝒰₀ where
    --   this : {k : K} -> {t : TermO σ V k} -> ∀{n} -> {ks : Vec K n} -> {ts : TermsO σ V ks} -> t ⊏-TermsO (t ∷ ts)
    --   _∷_ : {k₁ k₂ : K} -> {t₁ : TermO σ V k₁} -> (t₂ : TermO σ V k₂)-> ∀{n} -> {ks : Vec K n} -> {ts : TermsO σ V ks} -> t₁ ⊏-TermsO ts -> t₁ ⊏-TermsO (t₂ ∷ ts)

    -- data _⊏O_ : {k₁ k₂ : K} -> (t₁ : TermO σ V k₁) -> (t₂ : TermO σ V k₂) -> 𝒰₀ where
    --   te : {k : K} -> {t : TermO σ V k} -> ∀{n} -> {ks : Vec K (suc n)} -> {s : σ k ks} -> {ts : TermsO σ V ks} -> (t ⊏-TermsO ts) -> t ⊏O te s (ts)

    _⊏'_ : (t s : ∑ Term σ V) -> 𝒰₀
    _⊏'_ (_ , t) (_ , s) = t ⊏ s

    depth-Term : ∀{k} -> Term σ V k -> ℕ
    depth-Terms : ∀{ks : Vec K n} -> Terms σ V ks -> Vec ℕ n
    depth-Termᵥ : ∀{k} -> Termᵥ σ V k -> ℕ
    depth-Termsᵥ : ∀{ks : Vec K n} -> Termsᵥ σ V ks -> Vec ℕ n

    depth-Termᵥ (te s ts) = suc (⋁ (depth-Termsᵥ ts))
    depth-Termᵥ (var x) = 0

    depth-Termsᵥ (t ∷ ts) = depth-Termᵥ t ∷ depth-Terms ts
    depth-Termsᵥ (fail∷ ts) = 0 ∷ depth-Termsᵥ ts

    depth-Terms [] = []
    depth-Terms (t ∷ ts) = depth-Term t ∷ depth-Terms ts

    depth-Term (te s ts) = suc (⋁ (depth-Termsᵥ ts))
    depth-Term (var x) = 0
    depth-Term fail = 0

    depth-forget : ∀{k} -> (t : Termᵥ σ V k) -> depth-Term (forget-Term t) ≡ depth-Termᵥ t
    depth-forget (te s ts) = refl
    depth-forget (var x) = refl

    depth-⊏-Terms : {k : K} -> ∀{n} -> {ks : Vec K n} -> {t : Term σ V k} -> {ts : Terms σ V ks}
                    -> t ⊏-Terms ts -> depth-Term t ≤ ⋁ (depth-Terms ts)
    depth-⊏-Terms {ts = .(_ ∷ _)} this = ι₀-∨ {A = ℕ}
    depth-⊏-Terms {ts = .(t₂ ∷ _)} (t₂ ∷ x) = trans-≤ {A = ℕ} (depth-⊏-Terms x) (ι₁-∨ {A = ℕ} {a = depth-Term t₂})

    depth-⊏-Termsᵥ : {k : K} -> ∀{n} -> {ks : Vec K n} -> {t : Term σ V k} -> {ts : Termsᵥ σ V ks}
                    -> t ⊏-Terms (forget-Terms ts) -> depth-Term t ≤ ⋁ (depth-Termsᵥ ts)
    depth-⊏-Termsᵥ {ts = t ∷ ts} this = trans-≤ {A = ℕ} (0 , depth-forget t) (ι₀-∨ {A = ℕ})
    depth-⊏-Termsᵥ {ts = x₁ ∷ ts} (.(forget-Term x₁) ∷ x) = trans-≤ {A = ℕ} (depth-⊏-Terms x) (ι₁-max {a = depth-Termᵥ x₁})
    depth-⊏-Termsᵥ {ts = fail∷ ts} this = zero-≤
    depth-⊏-Termsᵥ {ts = fail∷ ts} (.fail ∷ x) = trans-≤ {A = ℕ} (depth-⊏-Termsᵥ x) (ι₁-max {a = 0})


    -- depth-⊏-Termsᵥ {ts = .(t ∷ _)} (this t _ x) = {!!}
    -- depth-⊏-Termsᵥ {ts = .(t₂ ∷ _)} (older t₂ x) = {!!}
    -- depth-⊏-Termsᵥ {ts = .(fail∷ _)} (fail∷ P) = {!!}

    private

      -- lem-10-Terms : ∀{n} {ks : Vec K n} -> (x : Terms σ V ks) -> Acc (_⊏'_) (_ , x)

      lem-10 : ∀{k} -> (x : Term σ V k) -> (n : ℕ) -> (depth-Term x ≤ n) -> Acc (_⊏'_) (_ , x)
      lem-10 (te s ts) zero P = 𝟘-rec (¬-<-zero P)
      lem-10 (te s ts) (suc n) P =
        acc (λ { (k , t') (te x) → lem-10 t' n (trans-≤ {A = ℕ} (depth-⊏-Termsᵥ x) (pred-≤-pred P))
               ;  (fst₁ , .fail) (fail a) → acc (λ { (fst₁ , .fail) (fail x) → 𝟘-rec (x refl)})
               })

      lem-10 (var x) n P = acc (λ { (fst₁ , .fail) (fail a) → acc (λ { (fst₁ , .fail) (fail x) → 𝟘-rec (x refl)})})
      lem-10 fail n P = acc (λ { (fst₁ , .fail) (fail a) → acc (λ { (fst₁ , .fail) (fail x) → 𝟘-rec (x refl)})})
      -- acc (λ {x y -> {!!}})

      -- lem-10 (t) = acc (λ { (k , snd₁) (te (this t .snd₁ x)) → {!!}
      --                     ; (k , snd₁) (te (older t₂ x)) → {!!}
      --                     ; (k , snd₁) (te (fail∷ x)) → {!!}})

      -- lem-10 (te s (fail∷ ts)) = acc (λ { (fst , .fail) (te this) → lem-10 fail
      --                                   ; (fst , snd₁) (te (.fail ∷ x)) → {!!}})
      -- -- acc (λ { (_ , t') (te x) → {!!}})
      -- lem-10 (var x) = acc (λ { y ()})
      -- lem-10 (fail) = acc (λ { y ()})

    isWellfounded::⊏ : WellFounded (λ (x y : ∑ Term σ V) -> x .snd ⊏ y .snd)
    isWellfounded::⊏ (_ , x) = lem-10 x (depth-Term x) refl-≤-ℕ

    {-

    _⊏O'_ : (t s : ∑ TermO σ V) -> 𝒰₀
    _⊏O'_ (_ , t) (_ , s) = t ⊏O s

    private
      -- lem-20-Terms : ∀{n} -> ∀{ks : Vec K n} -> (x : TermsO σ V ks) -> Acc (_)
      -- {-# INLINE lem-20 #-}

      postulate
        use : ∀{A B : 𝒰₀} -> A -> B
      -- use = {!!}
      acc-te : ∀{n}-> ∀{ks : Vec K (suc n)} -> (ts : TermsO σ V ks) -> (∀{k} (t : TermO σ V k)
             -> t ⊏-TermsO ts -> Acc (_⊏O'_) (_ , t)) -> ∀ {j} -> ∀(s : σ j (ks)) -> Acc (_⊏O'_) (_ , te s ts)
      acc-te = {!!}

      lem-20 : ∀{k} -> (x : TermO σ V k) -> Acc (_⊏O'_) (_ , x)

      lem-21 : ∀{n}-> ∀{ks : Vec K n} -> (ts : TermsO σ V ks) -> ∀{k} (t : TermO σ V k) -> t ⊏-TermsO ts -> Acc (_⊏O'_) (_ , t)
      lem-21 .(t ∷ _) t this = lem-20 t
      lem-21 .(t₂ ∷ _) t (t₂ ∷ p) = {!!}
      -- lem-21 .(t ∷ _) t this = 
      -- lem-21 .(t₂ ∷ _) t (t₂ ∷ p) = lem-21 t _ p

      -- lem-20 (te s ts) = acc-te ts (lem-21 ts) s
      lem-20 (te s (t ∷ [])) = use (lem-20 t)
      lem-20 (te s (t ∷ (t₁ ∷ ts))) = {!!}
      lem-20 (var x) = acc (λ { y ()})
      lem-20 fail = acc (λ { y ()})

      {-# INLINE lem-21 #-}
      -}

      -- lem-20 (te s (t ∷ [])) = use f -- acc (λ { (_ , t') (te this) → f})
      --   where f = lem-20 t
      -- lem-20 (te s (t ∷ (t₁ ∷ ts))) = {!!}
      -- -- acc (λ {y (te x) → lem-21 _ ts x})
      -- lem-20 (var x) = acc (λ { y ()})
      -- lem-20 fail = acc (λ { y ()})

      -- lem-20 (te s ts) = acc (λ {y (te x) → lem-21 _ ts x})
      -- lem-20 (var x) = acc (λ { y ()})
      -- lem-20 fail = acc (λ { y ()})



      -- acc (λ { (k , t') (te this) → {!!}
      --                   ; (k , t') (te (t₂ ∷ x)) → {!!}})
      {-
    forget-O-Terms : ∀{n} -> {ks : Vec K n} -> Termsᵥ σ V ks -> TermsO σ V ks
    forget-O-Terms (x ∷ ts) = {!!}
    forget-O-Terms (fail∷ ts) = {!!}

    forget-O-Term : ∀{k} -> Term σ V k -> TermO σ V k
    forget-O-Term (te s ts) = te s (forget-O-Terms ts)
    forget-O-Term (var x) = var x
    forget-O-Term fail = fail

    acc-O : ∀{k} -> ∀(x : Term σ V k) -> Acc _⊏O'_ (_ , forget-O-Term x) -> Acc _⊏'_ (_ , x)
    acc-O (te s ts) A = {!!}
    acc-O (var x) A = {!!}
    acc-O fail A = {!!}

    isWellfounded::⊏O : WellFounded (λ (x y : ∑ TermO σ V) -> x ⊏O' y)
    isWellfounded::⊏O (_ , x) = {!!}
    -}


    -- (_ , te s ts) = {!!}
    -- isWellfounded::⊏ (_ , var x) = {!!}
    -- isWellfounded::⊏ (_ , fail) = {!!}
-- acc (λ {(_ , y) y⊏x -> {!!}})

    fail⊏-Terms : {k : K} -> ∀{n} -> {ks : Vec K n} -> {t : Term σ V k} -> {ts : Terms σ V ks}
                -> t ⊏-Terms ts -> isFail-Terms ts -> isFail-Term t
    fail⊏-Terms this (x ∷ F) = x
    fail⊏-Terms (t₂ ∷ P) (x ∷ F) = fail⊏-Terms P F


    join-Term : {k : K} -> Term σ (Term σ V) k -> Term σ V k
    join-Termᵥ : {k : K} -> Termᵥ σ (Term σ V) k -> Term σ V k

    join-Terms : {ks : Vec K n} -> Terms σ (Term σ V) ks -> Terms σ V ks
    join-Terms [] = []
    join-Terms (t ∷ ts) = join-Term t ∷ join-Terms ts

    join-Termsᵥ : {ks : Vec K n} -> Termsᵥ σ (Term σ V) ks -> Terms σ V ks
    join-Termsᵥ (t ∷ ts) = join-Termᵥ t ∷ join-Terms ts
    join-Termsᵥ (fail∷ ts) = fail ∷ join-Termsᵥ ts

    reduce-Term : ∀{k} -> (t : Term σ V k) -> isFail-Term t +-𝒰 (∑ λ (t' : Termᵥ σ V k) -> forget-Term t' ≡ t)
    reduce-Term (te s ts) = right (te s ts , refl)
    reduce-Term (var x) = right (var x , refl)
    reduce-Term fail = left fail

    reduce-Terms : {ks : Vec K n} -> (ts : Terms σ V ks) -> (isFail-Terms ts) +-𝒰 (∑ λ (ts' : Termsᵥ σ V ks) -> forget-Terms ts' ≡ ts)
    reduce-Terms [] = left []
    reduce-Terms (t ∷ ts) with reduce-Term t
    ... | just (t' , t'P) = right (t' ∷ ts , λ i -> t'P i ∷ ts)
    ... | left fail with reduce-Terms ts
    ... | left (ts'F) = left (fail ∷ ts'F)
    ... | just (ts' , ts'P) = right (fail∷ ts' , λ i -> fail ∷ ts'P i)

    join-te : ∀{k} {ks : Vec K (suc n)} -> σ k ks -> Terms σ V ks -> Term σ V k
    join-te s ts with split-+-Str (reduce-Terms ts)
    ... | left (_ , _) = fail
    ... | just ((ts' , _) , _) = te s ts'

    join-Termᵥ (te s ts) = join-te s (join-Termsᵥ ts)
    join-Termᵥ (var x) = x

    join-Term (te s ts) = join-te s (join-Termsᵥ ts)
    join-Term (var t) = t
    join-Term fail = fail

  module _ {σ : Signature} {V : K -> 𝒰₀} where
    join⊏-Terms : {ks : Vec K n} -> ∀{k} -> {t : Term σ (Term σ V) k} {ts : Terms σ (Term σ V) ks} -> t ⊏-Terms ts -> join-Term t ⊏-Terms join-Terms ts
    join⊏-Terms {t = t} {.(t ∷ _)} this = this
    join⊏-Terms {t = t} {.(t₂ ∷ _)} (t₂ ∷ P) = _ ∷ join⊏-Terms P

    split:join∣forget-Term : ∀{k} -> (t : Termᵥ σ (Term σ V) k) -> join-Termᵥ t ≡ join-Term (forget-Term t)
    split:join∣forget-Term (te s ts) = refl
    split:join∣forget-Term (var x) = refl

    split:join∣forget-Terms : {ks : Vec K n} -> (ts : Termsᵥ σ (Term σ V) ks) -> join-Termsᵥ ts ≡ join-Terms (forget-Terms ts)
    split:join∣forget-Terms (t ∷ ts) i = split:join∣forget-Term t i ∷ join-Terms ts
    split:join∣forget-Terms (fail∷ ts) i = fail ∷ split:join∣forget-Terms ts i

    reduce-isFail-Term : ∀{k} -> {t : Term σ V k} -> isFail-Term t -> ∑ λ x -> reduce-Term t ≡-Str left x
    reduce-isFail-Term fail = _ , refl

    reduce-isFail-Terms : {ks : Vec K n} -> {ts : Terms σ V ks} -> isFail-Terms ts -> ∑ λ x -> reduce-Terms ts ≡-Str left x
    reduce-isFail-Terms {ts = .[]} [] = _ , refl
    reduce-isFail-Terms {ts = (t ∷ ts)} (x ∷ P) with reduce-Term t | reduce-isFail-Term x
    ... | left fail | .fail , refl-StrId with reduce-Terms ts | reduce-isFail-Terms P
    ... | left x₁ | Y = _ , refl


  module _ (σ : Signature) where
    IdxTerm : IdxSet K ℓ₀ -> IdxSet K ℓ₀
    ⟨ IdxTerm V ⟩ = Term σ ⟨ V ⟩
    of (IdxTerm V) = {!!}

  module _ {σ : Signature} where
    instance
      IdxSet:IdxTerm : {A : K -> 𝒰₀} -> {{_ : IIdxSet K A}} -> IIdxSet K (Term σ A)
      IdxSet:IdxTerm {A} {{_}} = of IdxTerm σ ` A `

  -- instance
  --   IdxSet:IdxTerm⇈ : {A : K -> 𝒰₀} -> {{_ : IIdxSet K A}} -> IIdxSet K (⇈ A)
  --   IdxSet:IdxTerm⇈ {A} = of _+-IdxSet_ 𝟙 ` A `
  -- = #openstruct IdxTerm


  module _ {σ : Signature} {V W : K -> 𝒰₀} where
    map-Term : {k : K} -> (∀{k} -> V k -> W k) -> Term σ V k -> Term σ W k
    map-Termᵥ : {k : K} -> (∀{k} -> V k -> W k) -> Termᵥ σ V k -> Termᵥ σ W k
    map-Terms : {ks : Vec K n} -> (∀{k} -> V k -> W k) -> Terms σ V ks -> Terms σ W ks
    map-Termsᵥ : {ks : Vec K n} -> (∀{k} -> V k -> W k) -> Termsᵥ σ V ks -> Termsᵥ σ W ks

    map-Termᵥ f (te s ts) = te s (map-Termsᵥ f ts)
    map-Termᵥ f (var x) = var (f x)

    map-Terms f [] = []
    map-Terms f (t ∷ ts) = map-Term f t ∷ map-Terms f ts

    map-Termsᵥ f (t ∷ ts) = map-Termᵥ f t ∷ map-Terms f ts
    map-Termsᵥ f (fail∷ ts) = fail∷ map-Termsᵥ f ts

    map-Term f (te s ts) = te s (map-Termsᵥ f ts)
    map-Term f (var x) = var (f x)
    map-Term f fail = fail


    commutes:map∣forget-Term : ∀{k} -> (f : ∀{k} -> V k -> W k) -> (t : Termᵥ σ V k) -> map-Term f (forget-Term t) ≡ (forget-Term (map-Termᵥ f t))
    commutes:map∣forget-Term f (te s ts) = refl
    commutes:map∣forget-Term f (var x) = refl

    commutes:map∣forget-Terms : {ks : Vec K n} -> (f : ∀{k} -> V k -> W k) -> (ts : Termsᵥ σ V ks) -> map-Terms f (forget-Terms ts) ≡ (forget-Terms (map-Termsᵥ f ts))
    commutes:map∣forget-Terms f (x ∷ ts) i = commutes:map∣forget-Term f x i ∷ map-Terms f ts
    commutes:map∣forget-Terms f (fail∷ ts) i = fail ∷ commutes:map∣forget-Terms f ts i

    map⊏-Terms : {ks : Vec K n} -> (f : ∀{k} -> V k -> W k) -> ∀{k} -> {t : Term σ V k} {ts : Terms σ V ks} -> t ⊏-Terms ts -> map-Term f t ⊏-Terms map-Terms f ts
    map⊏-Terms f {k} {t} {.(t ∷ _)} this = this
    map⊏-Terms f {k} {t} {.(t₂ ∷ _)} (t₂ ∷ P) = _ ∷ map⊏-Terms f P

    mapIsFail-Terms : {ks : Vec K n} -> (f : ∀{k} -> V k -> W k) -> {ts : Terms σ V ks} -> isFail-Terms ts -> isFail-Terms (map-Terms f ts)
    mapIsFail-Terms f [] = []
    mapIsFail-Terms f (fail ∷ P) = fail ∷ mapIsFail-Terms f P

    map⁻¹-IsFail-Term : ∀{k} -> (f : ∀{k} -> V k -> W k) -> {t : Term σ V k} -> isFail-Term (map-Term f t) -> isFail-Term t
    map⁻¹-IsFail-Term f {t = fail} P = fail

    map⁻¹-IsFail-Terms : {ks : Vec K n} -> (f : ∀{k} -> V k -> W k) -> {ts : Terms σ V ks} -> isFail-Terms (map-Terms f ts) -> isFail-Terms ts
    map⁻¹-IsFail-Terms f {ts = []} P = []
    map⁻¹-IsFail-Terms f {ts = t ∷ ts} (x ∷ P) = map⁻¹-IsFail-Term f x ∷ map⁻¹-IsFail-Terms f P


  module _ {σ : Signature} {V : K -> 𝒰₀} where

    functoriality-id:map-Term : {k : K} -> (t : Term σ V k) -> map-Term id t ≡ t
    functoriality-id:map-Termᵥ : {k : K} -> (t : Termᵥ σ V k) -> map-Termᵥ id t ≡ t
    functoriality-id:map-Termsᵥ : {ks : Vec K n} -> (ts : Termsᵥ σ V ks) -> map-Termsᵥ id ts ≡ ts

    functoriality-id:map-Termᵥ (te s ts) i = te s (functoriality-id:map-Termsᵥ ts i)
    functoriality-id:map-Termᵥ (var x) = refl

    functoriality-id:map-Terms : {ks : Vec K n} -> (ts : Terms σ V ks) -> map-Terms id ts ≡ ts
    functoriality-id:map-Terms [] = refl
    functoriality-id:map-Terms (t ∷ ts) i = functoriality-id:map-Term t i ∷ functoriality-id:map-Terms ts i

    functoriality-id:map-Termsᵥ (x ∷ ts) i = functoriality-id:map-Termᵥ x i ∷ functoriality-id:map-Terms ts i
    functoriality-id:map-Termsᵥ (fail∷ ts) i = fail∷ (functoriality-id:map-Termsᵥ ts i)

    functoriality-id:map-Term (te s ts) i = te s (functoriality-id:map-Termsᵥ ts i)
    functoriality-id:map-Term (var x) = refl
    functoriality-id:map-Term fail = refl


    ------

  module _ {σ : Signature} {U V W : K -> 𝒰₀} where
    functoriality-◆:map-Term   : (g : ∀{k} -> U k -> V k) (f : ∀{k} -> V k -> W k) {k : K} -> (t : Term σ U k)            -> map-Term f (map-Term g t)    ≡ map-Term (g ◆ f) t
    functoriality-◆:map-Termᵥ  : (g : ∀{k} -> U k -> V k) (f : ∀{k} -> V k -> W k) {k : K} -> (t : Termᵥ σ U k)           -> map-Termᵥ f (map-Termᵥ g t)   ≡ map-Termᵥ (g ◆ f) t
    functoriality-◆:map-Terms  : (g : ∀{k} -> U k -> V k) (f : ∀{k} -> V k -> W k) {ks : Vec K n} -> (ts : Terms σ U ks)  -> map-Terms f (map-Terms g ts)  ≡ map-Terms (g ◆ f) ts
    functoriality-◆:map-Termsᵥ : (g : ∀{k} -> U k -> V k) (f : ∀{k} -> V k -> W k) {ks : Vec K n} -> (ts : Termsᵥ σ U ks) -> map-Termsᵥ f (map-Termsᵥ g ts) ≡ map-Termsᵥ (g ◆ f) ts

    functoriality-◆:map-Termᵥ g f (te s ts) i = te s (functoriality-◆:map-Termsᵥ g f ts i)
    functoriality-◆:map-Termᵥ g f (var x) = refl

    functoriality-◆:map-Terms g f [] = refl
    functoriality-◆:map-Terms g f (t ∷ ts) i = functoriality-◆:map-Term g f t i ∷ functoriality-◆:map-Terms g f ts i

    functoriality-◆:map-Termsᵥ g f (x ∷ ts) i = functoriality-◆:map-Termᵥ g f x i ∷ functoriality-◆:map-Terms g f ts i
    functoriality-◆:map-Termsᵥ g f (fail∷ ts) i = fail∷ (functoriality-◆:map-Termsᵥ g f ts i)

    functoriality-◆:map-Term g f (te s ts) i = te s (functoriality-◆:map-Termsᵥ g f ts i)
    functoriality-◆:map-Term g f (var x) = refl
    functoriality-◆:map-Term g f fail = refl

  module _ {σ : Signature} {V W : K -> 𝒰₀} where
    natural:join-te : (f : ∀{k} -> V k -> W k) {ks : Vec K (suc n)} -> ∀{k} -> (s : σ k ks) -> (ts : Terms σ V ks) -> map-Term f (join-te s ts) ≡ join-te s (map-Terms f ts)
    natural:join-te f s ts with split-+-Str (reduce-Terms ts) | split-+-Str (reduce-Terms (map-Terms f ts))
    ... | left x | left x₁ = refl
    ... | left (x , xP) | just ((y , yP) , yQ) =
      let x1 : isFail-Terms (map-Terms f ts)
          x1 = mapIsFail-Terms f x
      in 𝟘-rec (left≢right (` reduce-isFail-Terms x1 .snd ⁻¹ ∙ yQ `))
    ... | just ((x , xP) , xQ) | left (y , yP) =
      let y1 = map⁻¹-IsFail-Terms f y
      in 𝟘-rec (left≢right (` reduce-isFail-Terms y1 .snd ⁻¹ ∙ xQ `))
    ... | just ((x , xP) , xQ) | just ((y , yP) , yQ) with ≡→≡-Str xP
    ... | refl-StrId =
      let Q1 = forget-Terms y ≡⟨ yP ⟩
               map-Terms f (forget-Terms x) ≡⟨ commutes:map∣forget-Terms f x ⟩
               forget-Terms (map-Termsᵥ f x) ∎
          Q2 = isInjective:forget-Terms (≡→≡-Str Q1)
      in λ i -> te s (≡-Str→≡ Q2 (~ i))

    naturality:join-Term : (f : ∀{k} -> V k -> W k) {k : K} -> (t : Term σ (Term σ V) k) -> map-Term f (join-Term t) ≡ join-Term (map-Term (map-Term f) t)
    naturality:join-Termsᵥ : (f : ∀{k} -> V k -> W k) {ks : Vec K (suc n)} -> ∀{k} -> (s : σ k ks) -> (ts : Termsᵥ σ (Term σ V) ks) -> map-Term f (join-te s (join-Termsᵥ ts)) ≡ join-te s (join-Termsᵥ (map-Termsᵥ (map-Term f) ts))

    naturality:join-Termᵥ : (f : ∀{k} -> V k -> W k) {k : K} -> (t : Termᵥ σ (Term σ V) k) -> map-Term f (join-Termᵥ t) ≡ join-Termᵥ (map-Termᵥ (map-Term f) t)
    naturality:join-Termᵥ f (te s ts) = naturality:join-Termsᵥ f s ts
    naturality:join-Termᵥ f (var x) = refl

    naturality:join-Terms : (f : ∀{k} -> V k -> W k) {ks : Vec K (n)} -> (ts : Terms σ (Term σ V) ks) -> map-Terms f (join-Terms ts) ≡ join-Terms (map-Terms (map-Term f) ts)
    naturality:join-Terms f [] = refl
    naturality:join-Terms f (t ∷ ts) i = naturality:join-Term f t i ∷ naturality:join-Terms f ts i

    naturality:join-Termsᵥ2 : (f : ∀{k} -> V k -> W k) {ks : Vec K (n)} -> (ts : Termsᵥ σ (Term σ V) ks) -> map-Terms f (join-Termsᵥ ts) ≡ join-Termsᵥ (map-Termsᵥ (map-Term f) ts)
    naturality:join-Termsᵥ2 f (x ∷ ts) i = naturality:join-Termᵥ f x i ∷ naturality:join-Terms f ts i
    naturality:join-Termsᵥ2 f (fail∷ ts) i = fail ∷ naturality:join-Termsᵥ2 f ts i

    naturality:join-Termsᵥ f s ts = map-Term f (join-te s (join-Termsᵥ ts)) ≡⟨ natural:join-te f s (join-Termsᵥ ts) ⟩
                                    join-te s (map-Terms f (join-Termsᵥ ts)) ≡[ i ]⟨ join-te s (naturality:join-Termsᵥ2 f ts i) ⟩
                                    join-te s (join-Termsᵥ (map-Termsᵥ (map-Term f) ts)) ∎


-- with split-+-Str (reduce-Terms (join-Termsᵥ ts)) | split-+-Str (reduce-Terms (join-Termsᵥ (map-Termsᵥ (map-Term f) ts)))
--     ... | left x | left x₁ = refl
--     ... | left x | just x₁ = {!!}
--     ... | just x | left x₁ = {!!}
--     ... | just ((x , xP) , xQ) | just x₁ = {!!}


    naturality:join-Term f (te s ts) = naturality:join-Termsᵥ f s ts
    naturality:join-Term f (var t) = refl
    naturality:join-Term f fail = refl

module _ {K : 𝒰₀} where
  module _ {σ : Signature} {V : K -> 𝒰₀} where

    reduce-forget-Term : ∀{k} -> (t : Termᵥ σ V k) -> ∑ λ x -> reduce-Term (forget-Term t) ≡-Str right x
    reduce-forget-Term (te s ts) = _ , refl
    reduce-forget-Term (var x) = _ , refl

    ¬isFail-forget-Term : ∀{k} -> (t : Termᵥ σ V k) -> isFail-Term (forget-Term t) -> 𝟘-𝒰
    ¬isFail-forget-Term (te s ts) ()
    ¬isFail-forget-Term (var x) ()

    ¬isFail-forget-Terms : ∀{ks : Vec K n} -> (ts : Termsᵥ σ V ks) -> isFail-Terms (forget-Terms ts) -> 𝟘-𝒰
    ¬isFail-forget-Terms (x ∷ ts) (xP ∷ P) = ¬isFail-forget-Term x xP
    ¬isFail-forget-Terms (fail∷ ts) (_ ∷ P) = ¬isFail-forget-Terms ts P

    reduce-forget-Terms : ∀{ks : Vec K n} -> (ts : Termsᵥ σ V ks) -> ∑ λ x -> reduce-Terms (forget-Terms ts) ≡-Str right x
    reduce-forget-Terms (x ∷ ts) with reduce-Term (forget-Term x) | reduce-forget-Term x
    ... | just x₁ | Y = _ , refl
    reduce-forget-Terms (fail∷_ {k = k} ts) with reduce-Terms (forget-Terms ts)
    ... | left x = 𝟘-rec (¬isFail-forget-Terms _ x)
    ... | just x = _ , refl

    join-te-forget : ∀{ks : Vec K (suc n)} -> ∀{k} -> (s : σ k ks)-> (ts : Termsᵥ σ V ks) -> join-te s (forget-Terms ts) ≡ te s ts
    join-te-forget s ts with split-+-Str (reduce-Terms (forget-Terms ts))
    ... | left (x , xQ) = 𝟘-rec (¬isFail-forget-Terms _ x)
    ... | just ((x , xP) , xQ) with isInjective:forget-Terms (≡→≡-Str xP)
    ... | refl-StrId = refl

    unit-r-join-Term : ∀{k} -> (x : Term σ V k) -> join-Term (map-Term var x) ≡ x
    unit-r-join-Terms : ∀{ks : Vec K n} -> (ts : Terms σ V ks) -> join-Terms (map-Terms var ts) ≡ ts
    unit-r-join-Termᵥ : ∀{k} -> (x : Termᵥ σ V k) -> join-Termᵥ (map-Termᵥ var x) ≡ forget-Term x

    unit-r-join-Termsᵥ : ∀{ks : Vec K n} -> (ts : Termsᵥ σ V ks) -> join-Termsᵥ (map-Termsᵥ var ts) ≡ forget-Terms ts
    unit-r-join-Termsᵥ (x ∷ ts) i = unit-r-join-Termᵥ x i ∷ unit-r-join-Terms ts i
    unit-r-join-Termsᵥ (fail∷ ts) i = fail ∷ unit-r-join-Termsᵥ ts i

    unit-r-join-Terms [] = refl
    unit-r-join-Terms (t ∷ ts) i = unit-r-join-Term t i ∷ unit-r-join-Terms ts i

    unit-r-join-Termᵥ (te s ts) = join-te s (join-Termsᵥ (map-Termsᵥ var ts)) ≡[ i ]⟨ join-te s (unit-r-join-Termsᵥ ts i) ⟩
                                  join-te s (forget-Terms ts)                 ≡⟨ join-te-forget s ts ⟩
                                  te s ts                                     ∎
    unit-r-join-Termᵥ (var x) = refl

    unit-r-join-Term (te s ts) = join-te s (join-Termsᵥ (map-Termsᵥ var ts)) ≡[ i ]⟨ join-te s (unit-r-join-Termsᵥ ts i) ⟩
                                  join-te s (forget-Terms ts)                 ≡⟨ join-te-forget s ts ⟩
                                  te s ts                                     ∎
    unit-r-join-Term (var x) = refl
    unit-r-join-Term fail = refl


  private
    𝒞 : Category _
    𝒞 = Category:IdxSet K ℓ₀

  module _ (σ : Signature) where
    Functor:Term : Functor 𝒞 𝒞
    ⟨ Functor:Term ⟩ X = IdxTerm σ X
    -- ⟨ ⟨ Functor:Term ⟩ X ⟩ = Term σ ⟨ X ⟩
    -- IIdxSet.ISet:this (of ⟨ Functor:Term ⟩ z) = {!!}
    ⟨ IFunctor.map (of Functor:Term) f ⟩ = map-Term ⟨ f ⟩
    IFunctor.functoriality-id (of Functor:Term) = functoriality-id:map-Term
    IFunctor.functoriality-◆ (of Functor:Term) x = functoriality-◆:map-Term _ _ x ⁻¹
    IFunctor.functoriality-≣ (of Functor:Term) p x i = map-Term (funExt p i) x

    Monad:Term : Monad 𝒞
    ⟨ Monad:Term ⟩ = Functor:Term
    ⟨ IMonad.return (of Monad:Term) ⟩ x = (var x)
    ⟨ IMonad.join (of Monad:Term) ⟩ = join-Term
    INatural.naturality (IMonad.INatural:return (of Monad:Term)) f x = refl
    INatural.naturality (IMonad.INatural:join (of Monad:Term)) f x = naturality:join-Term ⟨ f ⟩ x
    IMonad.unit-l-join (of Monad:Term) x = refl
    IMonad.unit-r-join (of Monad:Term) x = unit-r-join-Term x
    IMonad.assoc-join (of Monad:Term) = {!!}

{-

    Functor:TermZ2 = Functor:EitherT 𝟙 (Monad:Term)
    Monad:TermZ2 = Monad:EitherT 𝟙 (Monad:Term)

    TermZ2 : (V : K -> 𝒰₀) -> K -> 𝒰₀
    TermZ2 V k = Term σ (⇈ V) k

    IdxTermZ2 : (V : IdxSet K ℓ₀) -> IdxSet K ℓ₀
    IdxTermZ2 V = IdxTerm σ (𝟙 + V)

    TermsZ2 : (V : K -> 𝒰₀) -> (Vec K n) -> 𝒰₀
    TermsZ2 V ks = Terms σ (⇈ V) ks

  module _ {σ : Signature} {V W : IdxSet K ℓ₀} where
    map-TermZ2 : {k : K} -> (V ⟶ W) -> TermZ2 σ ⟨ V ⟩ k -> TermZ2 σ ⟨ W ⟩ k
    map-TermZ2 {k} f = ⟨ map {{of Functor:TermZ2 σ}} f ⟩ {k}

    map-TermsZ2 : {ks : Vec K n} -> (V ⟶ W) -> TermsZ2 σ ⟨ V ⟩ ks -> TermsZ2 σ ⟨ W ⟩ ks
    map-TermsZ2 f = map-Terms (⟨ map-+-r {c = 𝟙} f ⟩ {_})

  module _ {σ : Signature} {V : IdxSet K ℓ₀} where
    join-TermZ2 : {k : K} -> TermZ2 σ (TermZ2 σ ⟨ V ⟩) k -> TermZ2 σ ⟨ V ⟩ k
    join-TermZ2 {k} x = ⟨ join {{of Monad:TermZ2 σ}} {A = V} ⟩ {k} x
-}
